extraction/examples/RustCounter.v
@@ -1,6 +1,7 @@
 From ConCert.Execution.Examples Require Counter.
-From ConCert.Extraction Require Import Common.
+From ConCert.Execution.Examples Require CounterSolana.
 From ConCert.Extraction Require Import ConcordiumExtract.
+From ConCert.Extraction Require Import Common.
 From ConCert.Extraction Require Import SolanaExtract.
 From ConCert.Extraction Require Import RustExtract.
 From Coq Require Import Bool.
@@ -9,10 +10,9 @@ From MetaCoq.Template Require Import All.
 
 Open Scope string.
 
-Definition COUNTER_MODULE1 : SolanaMod _ _ :=
-  {| solana_contract_name := "counter";
-     solana_init := @ConCert.Execution.Examples.Counter.counter_init;
-     solana_receive := @ConCert.Execution.Examples.Counter.counter_receive;
+Definition COUNTER_MODULE1 : SolanaMod _ :=
+  {| solana_contract_name := "Counter";
+     solana_process := @ConCert.Execution.Examples.CounterSolana.counter_process;
      solana_extra := []; |}.
 
 Definition COUNTER_MODULE : ConcordiumMod _ _ :=
@@ -28,19 +28,21 @@ Instance RustConfig : RustPrintConfig :=
        any_type_symbol := "()";
        print_full_names := false |}.
 
-Redirect "/home/johnny/Documents/Tese/ConCert/extraction/examples/extracted-code/concordium-extract/counterv2.rs"
+Redirect "/home/johnny/Documents/Tese/ConCert/extraction/examples/extracted-code/solana-extract/counterv2.rs"
 
 MetaCoq Run (solana_extraction
                COUNTER_MODULE1
                (SolanaRemap.build_remaps
-                  (SolanaRemap.remap_arith ++ SolanaRemap.remap_blockchain_consts)
+                  (SolanaRemap.remap_arith ++ SolanaRemap.remap_blockchain_consts (* ++ SolanaRemap.remap_aux_consts *))
                   []
                   (SolanaRemap.remap_blockchain_inductives
                      ++ SolanaRemap.remap_std_types))
                (fun kn => eq_kername <%% bool_rec %%> kn
                           || eq_kername <%% bool_rect %%> kn)).
 
-(* MetaCoq Run (concordium_extraction
+Redirect "/home/johnny/Documents/Tese/ConCert/extraction/examples/extracted-code/concordium-extract/counterv2.rs"
+
+MetaCoq Run (concordium_extraction
                COUNTER_MODULE
                (ConcordiumRemap.build_remaps
                   (ConcordiumRemap.remap_arith ++ ConcordiumRemap.remap_blockchain_consts)
@@ -48,4 +50,4 @@ MetaCoq Run (solana_extraction
                   (ConcordiumRemap.remap_blockchain_inductives
                      ++ ConcordiumRemap.remap_std_types))
                (fun kn => eq_kername <%% bool_rec %%> kn
-                          || eq_kername <%% bool_rect %%> kn)). *)
+                          || eq_kername <%% bool_rect %%> kn)).
